Update metacoq (#62)
Update for the new MetaCoq version that has a flag that decides whether
matches on boxes can be done. The new relation also requires information
about inductives to be present to determine whether matches are
propositional, so because of this our erasure also needed to change a
bit. In particular, trans_env now has a straightforward translation for
each declaration type.

This should allow us to use MetaCoq's box optimization in a follow-up
change.

extraction/theories/Erasure.v
@@ -1256,46 +1256,62 @@ erase_ind_ctor Γ erΓ t isT next_par (tvar :: tvars)
 Proof. all: reduce_term_sound; eauto with erase. Qed.
 
 Import ExAst.
-Program Definition erase_ind_body
+Definition erase_ind_body
         (mind : kername)
         (mib : P.mutual_inductive_body)
         (oib : P.one_inductive_body)
-        (wt : ∥∑i, on_ind_body (lift_typing typing) Σ mind mib i oib∥) : one_inductive_body :=
+        (wt : ∥∑i, on_ind_body (lift_typing typing) Σ mind mib i oib∥) : one_inductive_body.
+Proof.
+  unshelve refine (
+  let is_propositional :=
+      match destArity [] (ind_type oib) with
+      | Some (_, u) => Universe.is_prop u
+      | None => false
+      end in
   let oib_tvars := erase_ind_arity [] (P.ind_type oib) _ in
 
-  let '(Γ; erΓ) := arities_contexts mind (P.ind_bodies mib) in
+  let ctx := inspect (arities_contexts mind (P.ind_bodies mib)) in
 
   let ind_params := firstn (P.ind_npars mib) oib_tvars in
   let erase_ind_ctor (p : (ident × P.term) × nat) (is_in : In p (P.ind_ctors oib)) :=
-      let '((name, t), _) := p in
-      let bt := erase_ind_ctor Γ erΓ t _ 0 ind_params in
+      let bt := erase_ind_ctor (proj1_sig ctx).π1 (proj1_sig ctx).π2 p.1.2 _ 0 ind_params in
       let '(ctor_args, _) := decompose_arr bt in
-      (name, ctor_args) in
+      (p.1.1, ctor_args) in
 
   let ctors := map_In (P.ind_ctors oib) erase_ind_ctor in
 
+  let erase_ind_proj (p : ident × P.term) (is_in : In p (P.ind_projs oib)) :=
+      (p.1, TBox) (* todo *) in
+
+  let projs := map_In (P.ind_projs oib) erase_ind_proj in
+
   {| ind_name := P.ind_name oib;
+     ind_propositional := is_propositional;
+     ind_kelim := P.ind_kelim oib;
      ind_type_vars := oib_tvars;
      ind_ctors := ctors;
-     ind_projs := [] (* todo *) |}.
-Next Obligation.
-  destruct wt as [wt].
-  sq.
-  right.
-  exact (onArity wt.π2).
-Qed.
-Next Obligation.
-  destruct wt as [[ind_index wt]].
-  pose proof (onConstructors wt) as on_ctors.
-  unfold on_constructors in *.
-  induction on_ctors; [easy|].
-  destruct is_in as [->|later]; [|easy].
-  constructor.
-  destruct (on_ctype r) as (s & typ).
-  rewrite <- (arities_contexts_1 mind) in typ.
-  rewrite <- Heq_anonymous in typ.
-  now exists s.
-Qed.
+     ind_ctor_original_arities := map snd (P.ind_ctors oib);
+     ind_projs := projs |}).
+
+  - abstract (
+        destruct wt as [wt];
+        sq;
+        right;
+        exact (onArity wt.π2)).
+  - abstract (
+        destruct p as ((?&?)&?);
+        cbn in *;
+        destruct wt as [[ind_index wt]];
+        pose proof (onConstructors wt) as on_ctors;
+        unfold on_constructors in *;
+        induction on_ctors; [easy|];
+        destruct is_in as [->|later]; [|easy];
+        constructor;
+        destruct (on_ctype r) as (s & typ);
+        rewrite <- (arities_contexts_1 mind) in typ;
+        cbn in *;
+        now exists s).
+Defined.
 
 Program Definition erase_ind
         (kn : kername)
@@ -1309,7 +1325,7 @@ Next Obligation.
   destruct wt as [wt].
   constructor.
   exists i.
-  specialize (onInductives _ _ _ _ wt).
+  specialize (onInductives wt).
 
   change i with (0 + i).
   generalize 0 as n.
