extraction/theories/Extraction.v
@@ -1,10 +1,9 @@
 (* This file provides the main function for invoking our extraction. *)
 
-From ConCert.Execution Require Import Blockchain.
-From ConCert.Execution Require Import Serializable.
 From ConCert.Extraction Require Import ClosedAux.
 From ConCert.Extraction Require Import Common.
 From ConCert.Extraction Require Import Erasure.
+From ConCert.Extraction Require Import ExAst.
 From ConCert.Extraction Require Import Optimize.
 From ConCert.Extraction Require Import OptimizeCorrectness.
 From ConCert.Extraction Require Import ResultMonad.
